\documentclass[main]{subfiles}
\begin{document}
\section{Logistic Regression}
\label{sec:logistic_regression}
%%%%%%%%%%%%%%%%%%%%%%%%%%%%%%%%%%%%%%%%%%%%%%%%%%%%%%%%%%%%%%%%%%%%%%%%%%%%%%%

\subsection{}

For brevity, use the following shorthand:
\begin{center}
\begin{math}
	g_{\v{\theta}}^{(i)} = h_{\v{\theta}}(y^{(i)}x^{(i)})
\end{math}
\end{center}

The empirical loss for the logistic regression becomes:
\begin{center}
\begin{math}
	J(\theta) = -\frac{1}{m} \sum\limits_{k=1}^{m}
				\log(g_{\v{\theta}}^{(k)})
\end{math}
\end{center}

First order partial derivatives:
\begin{align*}
	\pd{J}{\theta_i}
		&=
			-\frac{1}{m} \sum\limits_{k=1}^{m}
			\frac{1}{g_{\v{\theta}}^{(k)}}
			\pd{g_{\v{\theta}}^{(k)}}{\theta_i} \\
		&=
			-\frac{1}{m} \sum\limits_{k=1}^{m}
			\frac{1 - g_{\v{\theta}}^{(k)}}{g_{\v{\theta}}^{(k)}}
			\pd{} {\theta_i} (
				y^{(k)}\v{\theta}\cdot \v{x}^{(k)}
			)									\\
		&=
			-\frac{1}{m} \sum\limits_{k=1}^{m}
			\frac{1 - g_{\v{\theta}}^{(k)}}{g_{\v{\theta}}^{(k)}}
			y^{(k)}x^{(k)}_i
\end{align*}

Compute the second order partial derivatives;
\begin{align*}
	\pdm{J}{\theta_i}{\theta_j}
		&=
			-\frac{1}{m} \sum\limits_{k=1}^{m}
			y^{(k)}x^{(k)}_i
			\pd{}{\theta_j} (
				\frac{1 - g_{\v{\theta}}^{(k)}}{g_{\v{\theta}}^{(k)}}
			)									\\
		&=
			\frac{1}{m} \sum\limits_{k=1}^{m}
			\frac{1}{(g_{\v{\theta}}^{(k)})^2}
			y^{(k)}x^{(k)}_i
			y^{(k)}x^{(k)}_j					\\
		&=
			\frac{1}{m} \sum\limits_{k=1}^{m}
			\Big(\frac{y^{(k)}}{g_{\v{\theta}}^{(k)}}\Big)^2
			 x^{(k)}_i x^{(k)}_j
\end{align*}

Therefore, the dual form is always non-negative:
\begin{align*}
	\sum\limits_{i,j} z_i H_{ij} z_j
		&=
			\sum\limits_{i,j}
			\frac{1}{m} \sum\limits_{k=1}^{m}
			\Big(\frac{y^{(k)}}{g_{\v{\theta}}^{(k)}}\Big)^2
			 z_i x^{(k)}_i z_j x^{(k)}_j		\\
		&=
			\frac{1}{m} \sum\limits_{k=1}^{m}
			\Big(\frac{y^{(k)}}{g_{\v{\theta}}^{(k)}}\Big)^2
			\sum\limits_{i}
			z_i x^{(k)}_i
			\sum\limits_{j}
			z_j x^{(k)}_j						\\
		&=
			\frac{1}{m} \sum\limits_{k=1}^{m}
			\Big(\frac{y^{(k)}}{g_{\v{\theta}}^{(k)}}\Big)^2
			(\v{z}\cdot\v{x})^2					\\
		&\geqslant 0
\end{align*}

\subsection{}
skipped

\subsection{}
skipped

%%%%%%%%%%%%%%%%%%%%%%%%%%%%%%%%%%%%%%%%%%%%%%%%%%%%%%%%%%%%%%%%%%%%%%%%%%%%%%%%
\end{document}
